src/MicroSail/Sep/Spec.v
@@ -31,6 +31,7 @@ From Coq Require
 
 From MicroSail Require Import
      Notation
+     Sep.Logic
      Syntax.
 
 Import CtxNotations.
@@ -180,6 +181,50 @@ Module Assertions
     Global Coercion sep_contract_pun_to_sep_contract : SepContractPun >-> SepContract.
 
   End Experimental.
+
+  Class IHeaplet (L : Type) := {
+    is_ISepLogic :> ISepLogic L;
+    lpred (p : 𝑷) (ts : Env Lit (𝑷_Ty p)) : L;
+    lptsreg  {σ : Ty} (r : 𝑹𝑬𝑮 σ) (t : Lit σ) : L
+  }.
+
+  Arguments lpred {L _} p ts.
+
+  Section Contracts.
+    Context `{Logic : IHeaplet L}.
+
+    Definition inst_chunk {Σ} (ι : SymInstance Σ) (c : Chunk Σ) : L :=
+      match c with
+      | chunk_pred p ts => lpred p (env_map (fun _ => inst_term ι) ts)
+      | chunk_ptsreg r t => lptsreg r (inst_term ι t)
+      end.
+
+    Fixpoint inst_assertion {Σ} (ι : SymInstance Σ) (a : Assertion Σ) : L :=
+      match a with
+      | asn_bool b => if inst_term ι b then emp else lfalse
+      | asn_prop p => !!(uncurry_named p ι) ∧ emp
+      | asn_chunk c => inst_chunk ι c
+      | asn_if b a1 a2 => if inst_term ι b then inst_assertion ι a1 else inst_assertion ι a2
+      | asn_match_enum E k alts => inst_assertion ι (alts (inst_term ι k))
+      | asn_sep a1 a2 => inst_assertion ι a1 ✱ inst_assertion ι a2
+      | asn_exist ς τ a => ∃ v, @inst_assertion (Σ ▻ (ς , τ)) (ι ► (ς , τ) ↦ v) a
+    end%logic.
+
+    Definition inst_contract_localstore {Δ τ} (c : SepContract Δ τ)
+      (ι : SymInstance (sep_contract_logic_variables c)) : LocalStore Δ :=
+      inst_localstore ι (sep_contract_localstore c).
+
+    Definition inst_contract_precondition {Δ τ} (c : SepContract Δ τ)
+      (ι : SymInstance (sep_contract_logic_variables c)) : L :=
+      inst_assertion ι (sep_contract_precondition c).
+
+    Definition inst_contract_postcondition {Δ τ} (c : SepContract Δ τ)
+      (ι : SymInstance (sep_contract_logic_variables c)) (result : Lit τ) :  L :=
+        inst_assertion (env_snoc ι (sep_contract_result c,τ) result) (sep_contract_postcondition c).
+
+  End Contracts.
+
+  Arguments inst_assertion {_ _ _} _ _.
 
 End Assertions.
 
